Semantics/FunctionalUtils.v
@@ -1,42 +1,43 @@
 From Coq Require Import List.
-From Warblre Require Import Base.
+From Warblre Require Import Base RegExpRecord.
 From Linden Require Import Regex Chars Groups Tree Semantics FunctionalSemantics ComputeIsTree.
 Import ListNotations.
 
 Section Utilities.
   Context {char: Parameters.Character.class}.
   Context {unicodeProp: Parameters.Property.class Parameters.Character}.
+  Context (rer: RegExpRecord).
 
   Definition compute_tr (act: actions) (inp: input) (gm: group_map) (dir: Direction): tree :=
-    match compute_tree act inp gm dir (S (actions_fuel act inp dir)) with
+    match compute_tree rer act inp gm dir (S (actions_fuel act inp dir)) with
     | Some tr => tr
     | None => Mismatch
     end.
 
   Lemma compute_tr_is_tree {actions i gm dir} :
-    is_tree actions i gm dir (compute_tr actions i gm dir).
+    is_tree rer actions i gm dir (compute_tr actions i gm dir).
   Proof.
     unfold compute_tr.
-    pose proof functional_terminates actions i gm dir _ (PeanoNat.Nat.lt_succ_diag_r _).
+    pose proof functional_terminates rer actions i gm dir _ (PeanoNat.Nat.lt_succ_diag_r _).
     destruct compute_tree eqn:Htr; try contradiction.
     eauto using compute_is_tree.
   Qed.
 
   Lemma compute_tr_reg_is_tree {r i gm dir} :
-    is_tree [Areg r] i gm dir (compute_tr [Areg r] i gm dir).
+    is_tree rer [Areg r] i gm dir (compute_tr [Areg r] i gm dir).
   Proof.
     eauto using compute_tr_is_tree.
   Qed.
 
   Lemma is_tree_eq_compute_tr {actions i gm dir} :
-    forall {tr}, is_tree actions i gm dir tr -> tr = compute_tr actions i gm dir.
+    forall {tr}, is_tree rer actions i gm dir tr -> tr = compute_tr actions i gm dir.
   Proof.
     eauto using is_tree_determ, compute_tr_is_tree.
   Qed.
 
   Lemma compute_tr_ind {actions i gm dir P} :
     P (compute_tr actions i gm dir) ->
-    forall {tr}, is_tree actions i gm dir tr -> P tr.
+    forall {tr}, is_tree rer actions i gm dir tr -> P tr.
   Proof.
     intros HP tr Htr.
     erewrite is_tree_determ with (1 := Htr) (2 := compute_tr_is_tree).
@@ -45,7 +46,7 @@ Section Utilities.
 
   Lemma compute_tr_reg_ind {r i gm dir P} :
     P (compute_tr [Areg r] i gm dir) ->
-    forall {tr}, is_tree [Areg r] i gm dir tr -> P tr.
+    forall {tr}, is_tree rer [Areg r] i gm dir tr -> P tr.
   Proof.
     intros; eapply compute_tr_ind; eauto.
   Qed.
@@ -68,7 +69,7 @@ Section Utilities.
     | Areg Epsilon::cont => compute_tr cont inp gm dir
     (* tree_char, tree_char_fail *)
     | Areg (Regex.Character cd)::cont =>
-        match read_char cd inp dir with
+        match read_char rer cd inp dir with
         | Some (c, nextinp) =>
             let treecont := compute_tr cont nextinp gm dir in
             Read c treecont
@@ -114,14 +115,14 @@ Section Utilities.
           LKFail lk treelk
     (* tree_anchor, tree_anchor_fail *)
     | Areg (Anchor a)::cont =>
-        if anchor_satisfied a inp then
+        if anchor_satisfied rer a inp then
           let treecont := compute_tr cont inp gm dir in
           AnchorPass a treecont
         else
           Mismatch
     (* tree_backref, tree_backref_fail *)
     | Areg (Backreference gid)::cont =>
-        match read_backref gm gid inp dir with
+        match read_backref rer gm gid inp dir with
         | Some (br_str, nextinp) =>
             let tcont := compute_tr cont nextinp gm dir in
             ReadBackRef br_str tcont
@@ -131,8 +132,8 @@ Section Utilities.
     end.
 
   Lemma compute_tree_None_compute_tr act inp gm dir fuel:
-    compute_tree act inp gm dir fuel <> None ->
-    compute_tree act inp gm dir fuel = Some (compute_tr act inp gm dir).
+    compute_tree rer act inp gm dir fuel <> None ->
+    compute_tree rer act inp gm dir fuel = Some (compute_tr act inp gm dir).
   Proof.
     intros HNone; destruct compute_tree eqn:Htr in *; [ | congruence ].
     apply compute_is_tree in Htr.
@@ -141,14 +142,14 @@ Section Utilities.
 
   Lemma compute_tree_compute_tr act inp gm dir:
     let fuel := S (actions_fuel act inp dir) in
-    compute_tree act inp gm dir fuel = Some (compute_tr act inp gm dir).
+    compute_tree rer act inp gm dir fuel = Some (compute_tr act inp gm dir).
   Proof.
     unfold compute_tr.
-    pose proof functional_terminates act inp gm dir _ (PeanoNat.Nat.lt_succ_diag_r _).
+    pose proof functional_terminates rer act inp gm dir _ (PeanoNat.Nat.lt_succ_diag_r _).
     destruct compute_tree; congruence.
   Qed.
 
-  Arguments compute_tree characterClass unicodeProp !act inp gm dir fuel.
+  Arguments compute_tree characterClass unicodeProp rer !act inp gm dir fuel.
 
   Lemma compute_tr_rw act inp gm dir:
     compute_tr act inp gm dir = compute_tr_unfold act inp gm dir.
@@ -159,84 +160,84 @@ Section Utilities.
     { reflexivity. }
     destruct act.
     - destruct r.
-      + set (treecont_opt := compute_tree cont inp gm dir _) in *.
+      + set (treecont_opt := compute_tree rer cont inp gm dir _) in *.
         assert (treecont_opt <> None). { destruct treecont_opt; discriminate. }
         apply compute_tree_None_compute_tr in H. fold treecont_opt in H.
         rewrite H in *. reflexivity.
       + destruct read_char as [[c nextinp]|]. 2: reflexivity.
-        set (treecont_opt := compute_tree cont nextinp gm dir _) in *.
+        set (treecont_opt := compute_tree rer cont nextinp gm dir _) in *.
         assert (treecont_opt <> None). { destruct treecont_opt; discriminate. }
         apply compute_tree_None_compute_tr in H. fold treecont_opt in H.
         rewrite H in *. reflexivity.
-      + set (t1_opt := compute_tree (Areg r1 :: cont) inp gm dir (regex_fuel (Disjunction r1 r2) inp dir + actions_fuel cont inp dir)) in *.
+      + set (t1_opt := compute_tree rer (Areg r1 :: cont) inp gm dir (regex_fuel (Disjunction r1 r2) inp dir + actions_fuel cont inp dir)) in *.
         assert (t1_opt <> None). { destruct t1_opt; discriminate. }
         apply compute_tree_None_compute_tr in H. fold t1_opt in H.
         rewrite H in *.
-        set (t2_opt := compute_tree (Areg r2 :: cont) inp gm dir (regex_fuel (Disjunction r1 r2) inp dir + actions_fuel cont inp dir)) in *.
+        set (t2_opt := compute_tree rer (Areg r2 :: cont) inp gm dir (regex_fuel (Disjunction r1 r2) inp dir + actions_fuel cont inp dir)) in *.
         assert (t2_opt <> None). { destruct t2_opt; discriminate. }
         apply compute_tree_None_compute_tr in H0. fold t2_opt in H0.
         rewrite H0 in *. reflexivity.
-      + set (tr_opt := compute_tree _ inp gm dir _) in *.
+      + set (tr_opt := compute_tree rer _ inp gm dir _) in *.
         assert (tr_opt <> None). { destruct tr_opt; discriminate. }
         apply compute_tree_None_compute_tr in H. fold tr_opt in H.
         rewrite H in *. reflexivity.
       + destruct min as [|min'].
         * destruct delta as [[|n']|].
-          -- set (tr_opt := compute_tree cont inp gm dir _) in *.
+          -- set (tr_opt := compute_tree rer cont inp gm dir _) in *.
              assert (tr_opt <> None). { destruct tr_opt; discriminate. }
              apply compute_tree_None_compute_tr in H. fold tr_opt in H.
              rewrite H in *. reflexivity.
-          -- set (titer_opt := compute_tree _ inp _ dir _) in *.
+          -- set (titer_opt := compute_tree rer _ inp _ dir _) in *.
              assert (titer_opt <> None). { destruct titer_opt; discriminate. }
              apply compute_tree_None_compute_tr in H. fold titer_opt in H.
              rewrite H in *.
-             set (tskip_opt := compute_tree cont inp gm dir _) in *.
+             set (tskip_opt := compute_tree rer cont inp gm dir _) in *.
              assert (tskip_opt <> None). { destruct tskip_opt; discriminate. }
              apply compute_tree_None_compute_tr in H0. fold tskip_opt in H0.
              rewrite H0 in *. reflexivity.
-          -- set (titer_opt := compute_tree _ inp _ dir _) in *.
+          -- set (titer_opt := compute_tree rer _ inp _ dir _) in *.
              assert (titer_opt <> None). { destruct titer_opt; discriminate. }
              apply compute_tree_None_compute_tr in H. fold titer_opt in H.
              rewrite H in *.
-             set (tskip_opt := compute_tree cont inp gm dir _) in *.
+             set (tskip_opt := compute_tree rer cont inp gm dir _) in *.
              assert (tskip_opt <> None). { destruct tskip_opt; discriminate. }
              apply compute_tree_None_compute_tr in H0. fold tskip_opt in H0.
              rewrite H0 in *. reflexivity.
-        * set (titer_opt := compute_tree _ inp _ dir _) in *.
+        * set (titer_opt := compute_tree rer _ inp _ dir _) in *.
           assert (titer_opt <> None). { destruct titer_opt; discriminate. }
           apply compute_tree_None_compute_tr in H. fold titer_opt in H.
           rewrite H in *. reflexivity.
-      + set (treelk_opt := compute_tree [Areg r] inp gm _ _) in *.
+      + set (treelk_opt := compute_tree rer [Areg r] inp gm _ _) in *.
         assert (treelk_opt <> None). { destruct treelk_opt; discriminate. }
         apply compute_tree_None_compute_tr in H. fold treelk_opt in H.
         rewrite H in *.
         destruct lk_succeeds. 2: reflexivity.
         destruct lk_group_map as [gmlk|]. 2: reflexivity.
-        set (treecont_opt := compute_tree cont inp gmlk dir _) in *.
+        set (treecont_opt := compute_tree rer cont inp gmlk dir _) in *.
         assert (treecont_opt <> None). { destruct treecont_opt; discriminate. }
         apply compute_tree_None_compute_tr in H0. fold treecont_opt in H0.
         rewrite H0 in *. reflexivity.
-      + set (treecont_opt := compute_tree _ inp _ dir _) in *.
+      + set (treecont_opt := compute_tree rer _ inp _ dir _) in *.
         assert (treecont_opt <> None). { destruct treecont_opt; discriminate. }
         apply compute_tree_None_compute_tr in H. fold treecont_opt in H.
         rewrite H in *. reflexivity.
       + destruct anchor_satisfied. 2: reflexivity.
-        set (treecont_opt := compute_tree cont inp gm dir _) in *.
+        set (treecont_opt := compute_tree rer cont inp gm dir _) in *.
         assert (treecont_opt <> None). { destruct treecont_opt; discriminate. }
         apply compute_tree_None_compute_tr in H. fold treecont_opt in H.
         rewrite H in *. reflexivity.
       + destruct read_backref as [[br_str nextinp]|]. 2: reflexivity.
-        set (tcont_opt := compute_tree cont nextinp gm dir _) in *.
+        set (tcont_opt := compute_tree rer cont nextinp gm dir _) in *.
         assert (tcont_opt <> None). { destruct tcont_opt; discriminate. }
         apply compute_tree_None_compute_tr in H. fold tcont_opt in H.
         rewrite H in *. reflexivity.
-    - set (treecont_opt := compute_tree cont inp gm dir _) in *.
+    - set (treecont_opt := compute_tree rer cont inp gm dir _) in *.
       destruct StrictSuffix.is_strict_suffix.
       2: reflexivity.
       assert (treecont_opt <> None). { destruct treecont_opt; discriminate. }
       apply compute_tree_None_compute_tr in H. fold treecont_opt in H.
       rewrite H in *. reflexivity.
-    - set (treecont_opt := compute_tree cont inp _ dir _) in *.
+    - set (treecont_opt := compute_tree rer cont inp _ dir _) in *.
       assert (treecont_opt <> None). { destruct treecont_opt; discriminate. }
       apply compute_tree_None_compute_tr in H. fold treecont_opt in H.
       rewrite H in *. reflexivity.
@@ -244,26 +245,26 @@ Section Utilities.
 
   Definition compute_tr_dep (act: actions) (inp: input) (gm: group_map) (dir: Direction): tree :=
     let fuel := S (actions_fuel act inp dir) in
-    let opt := compute_tree act inp gm dir fuel in
+    let opt := compute_tree rer act inp gm dir fuel in
     match opt as o return opt = o -> tree with
     | Some tr =>
         fun _ => tr
     | None =>
-        fun Heq => False_rect _ (functional_terminates act inp gm dir fuel (PeanoNat.Nat.lt_succ_diag_r _) Heq)
+        fun Heq => False_rect _ (functional_terminates rer act inp gm dir fuel (PeanoNat.Nat.lt_succ_diag_r _) Heq)
     end eq_refl.
 
   Lemma compute_tr_dep_is_tree {actions i gm dir} :
-    is_tree actions i gm dir (compute_tr_dep actions i gm dir).
+    is_tree rer actions i gm dir (compute_tr_dep actions i gm dir).
   Proof.
     unfold compute_tr_dep.
-    set (functional_terminates _ _ _ _ _ _) as fn; clearbody fn.
+    set (functional_terminates _ _ _ _ _ _ _) as fn; clearbody fn.
     destruct compute_tree eqn:Htr; try contradiction.
     eauto using compute_is_tree.
   Qed.
 
   (* TODO compute_tr_dep_unfold?? *)
   Lemma compute_tr_dep_reg_is_tree {r i gm dir} :
-    is_tree [Areg r] i gm dir (compute_tr_dep [Areg r] i gm dir).
+    is_tree rer [Areg r] i gm dir (compute_tr_dep [Areg r] i gm dir).
   Proof.
     eauto using compute_tr_dep_is_tree.
   Qed.
